<h1><center>Chapter 2 : Euclidean Space </center></h1>

<b>Question 1</b><br>
Let $u = \begin{pmatrix} 
-1\\ 
3\\ 
\end{pmatrix}$ 
and 
$v = \begin{pmatrix} 
2\\ 
1\\ 
\end{pmatrix}$ be vector in $\mathbb{R}^2$. Evaluate the following: 


(a)$u\cdot v \quad $(b)$ v \cdot u \quad$ (c)$ u \cdot u\quad$ (d)$ v \cdot v\quad $ (e)$\lVert u \rVert^{2}$ <br>
(f)$\lVert v\rVert^{2}\quad$ (g)$\lVert u\rVert \quad $(h)$\lVert v \rVert\quad$(i)$\lVert u + v \rVert^{2}\quad $ (j)$d(u, v)\quad$

<b>Solution</b><br>
(a) -1(2) + 3(1) = 1 <br>
(b) since $u \cdot v = v \cdot u$. Therefore, $v \cdot u = 1$ <br>
(c) $u \cdot u = (-1)(-1) + 3(3) = 10$ <br>
(d) $v \cdot v = 2(2) + 1(1) = 5 $<br>
(e) $\lVert u \rVert^2 = u \cdot u = 10\quad$ From (c) <br>
(f) $\lVert v \rVert^2 = v \cdot v = 5\quad$ From (d) <br>
(g) $\lVert u \rVert = \sqrt{u \cdot u} = \sqrt{10}$<br>
(h) $\lVert v \rVert = \sqrt{v \cdot v} = \sqrt{5}$<br>
(i) $\lVert u + v \rVert^2 = (u + v) \cdot (u + v) = \begin{pmatrix}
1\\
4\\
\end{pmatrix}\cdot
\begin{pmatrix}
1\\
4\\
\end{pmatrix} = 1^2 + 4^2 = 17$ <br>
(j) $ d(u, v) = \lVert u - v \rVert = \lVert \begin{pmatrix}
-1\\
3\\
\end{pmatrix} -
\begin{pmatrix}
2\\
1\\
\end{pmatrix}\rVert = \lVert\begin{pmatrix}
-3\\
2\\
\end{pmatrix}
\rVert
 = \sqrt{(-3)^2 + 2^2} = \sqrt{13}$

----------------------------------------------------------------------------

<b>Question 2</b><br>
Let $u  = \begin{pmatrix} 
2&3&-1\\ 
\end{pmatrix}^T$ 
and 
$v = \begin{pmatrix} 
5&1&-2\\ 
\end{pmatrix}^T$ be vectors in $\mathbb{R}^{3}$. Evaluate: 


(a)$u\cdot v \quad $(b)$ v \cdot u \quad$ (c)$ u \cdot u\quad$ (d) $ v \cdot v\quad $ (e) $\lVert u \rVert^{2}$ <br>
(f)$\lVert v\rVert^{2}\quad$ (g)$\lVert u \rVert\quad $(h)$\lVert v \rVert\quad$(i)$\lVert u + v\rVert^{2}\quad $ (j)$d(u, v)\quad$

<b>Solution</b> <br>
Here, 
$u = \begin{pmatrix}
2\\
3\\
-1\\
\end{pmatrix}, v = \begin{pmatrix}
5\\
1\\
-2\\
\end{pmatrix}$ <br>
(a) $u \cdot v = 2(5) + 3(1) + (-1)2 = 15$ <br>
(b) $ u \cdot v = v \cdot u = 15$ <br>
(c) $ u \cdot u = 2(2) + 3(3) + (-1)(-1) = 14$ <br>
(d) $ v \cdot v = 5(5) + 1(1) + (-2)(-2) = 30$ <br>
(e) $ \lVert u \rVert^2 = u \cdot u = 14 \quad$ From(c) <br>
(f) $ \lVert v \rVert^2 = v \cdot v = 30 \quad$ From(d) <br>
(g) $ \lVert u \rVert = \sqrt{u \cdot u} = \sqrt{14}$ <br>
(h) $ \lVert v \rVert = \sqrt{v \cdot v} = \sqrt{30}$ <br> 
(i) $\lVert u + v \rVert^2 = (u + v) \cdot (u + v) = \begin{pmatrix}
7\\
4\\
-3\\
\end{pmatrix}
\cdot
\begin{pmatrix}
7\\
4\\
-3\\
\end{pmatrix}
= 7(7) + 4(4) + (-3)(-3) = 74$ <br>
(j) $d(u, v) = \lVert u - v \rVert = \lVert \begin{pmatrix}
-3\\
2\\
1\\
\end{pmatrix} \rVert = \sqrt{(-3)^2 + 2^2 + 1^2} = \sqrt{14}$

-----------------------------------------------------------------------

<b>Question 3</b><br>

Let $u  = \begin{pmatrix}
-1&2&5&-3\\
\end{pmatrix}^T$ and $v = \begin{pmatrix}
2&-3&-1&5\\
\end{pmatrix}^T$ be vectors in $\mathbb{R}^{3}$. Evaluate:


(a)$u\cdot v \quad $(b)$ v \cdot u \quad$ (c)$ u \cdot u\quad$ (d) $ v \cdot v\quad $ (e) $\lVert u \rVert^{2}$ <br>
(f)$\lVert v \rVert^{2}\quad$ (g)$\lVert u\rVert\quad $(h)$\lVert v \rVert\quad$(i)$\lVert u + v\rVert^{2}\quad $ (j)$d(u, v)\quad$

<b>Solution</b><br>
$ u = \begin{pmatrix}
-1\\
2\\
5\\
-3\\
\end{pmatrix}, v = \begin{pmatrix}
2\\
-3\\
-1\\
5\\
\end{pmatrix}$ <br>
(a) $(-1)(2) + 2(-3) + 5(-1) + (-3)(5) = -28$ <br>
(b) $ v \cdot u =  u \cdot v = -28$ <br>
(c) $ u \cdot u = -1(-1) + 2(2) + 5(5) + (-3)(-3) = 39$ <br>
(d) $ v \cdot v = 2(2) + (-3)(-3) + (-1)(-1) + 5(5) = 39$<br>
(e) $\lVert u \rVert^2 = u \cdot u = 39$ From (c)<br>
(f) $\lVert v \rVert^2 = v \cdot v = 39$ From (d)<br>
(g) $ \lVert u \rVert = \sqrt{u \cdot u} = \sqrt{39}$ <br>
(h) $ \lVert v \rVert = \sqrt{v \cdot v} = \sqrt{39}$ <br> 
(i) $\lVert u + v \rVert^2 = (u + v) \cdot (u + v) = \begin{pmatrix}
1\\
-1\\
4\\
2\\
\end{pmatrix} \cdot \begin{pmatrix}
1\\
-1\\
4\\
2\\
\end{pmatrix}
= 1(1) + (-1)(-1) + 4(4) + 2(2) = 22$ <br>
(j) $ d(u, v) = \lVert u - v \rVert = \lVert \begin{pmatrix}
-3\\
5\\
6\\
-8\\
\end{pmatrix} \rVert = \sqrt{(-3)^2 + (5)^2 + (6)^2 + (-8)^2} = \sqrt{134}$

---------------------------------------------------------------------------------------------

4. Let $i  = \begin{pmatrix}
1\\
0\\
0\\
\end{pmatrix}$, $j = \begin{pmatrix}
0\\
1\\
0\\
\end{pmatrix}$ and $k = \begin{pmatrix}
0\\
0\\
1\\
\end{pmatrix}$. Show that<br> 
(a) $i \cdot i = 1 \quad$(b) $j \cdot j = 1 \quad$(c) $k \cdot k = 1 \quad$(d) $i \cdot j = 0 \quad$<br>
(e) $i \cdot k = 0 \quad$(f) $j \cdot k = 0 \quad$<br>
If $u = ai + bj + ck$ and $di + ej + fk$ show that $ u \cdot v = ad +  be + cf$

<b>Solution </b><br>(a) $i \cdot i = \begin{pmatrix} 
1\\
0\\
0\\
\end{pmatrix}
\begin{pmatrix}
1\\
0\\
0\\
\end{pmatrix}
= 1 + 0 + 0 = 1\qquad $(b)$ j \cdot j = \begin{pmatrix} 
0\\
1\\
0\\
\end{pmatrix}
\begin{pmatrix}
0\\
1\\
0\\
\end{pmatrix}
= 0 + 1 + 0 = 1\qquad$(c)$ k \cdot k = \begin{pmatrix} 
0\\
0\\
1\\
\end{pmatrix}
\begin{pmatrix}
0\\
0\\
1\\
\end{pmatrix}
= 0 + 0 + 1 = 1\qquad$ <br>
(d) $i \cdot j = \begin{pmatrix} 
1\\
0\\
0\\
\end{pmatrix}
\begin{pmatrix}
0\\
1\\
0\\
\end{pmatrix}
= 0 + 0 + 0 = 0\qquad$ (e) $i \cdot k = \begin{pmatrix} 
1\\
0\\
0\\
\end{pmatrix}
\begin{pmatrix}
0\\
0\\
1\\
\end{pmatrix}
= 0 + 0 + 0 = 0\qquad$ (f) $j \cdot k = \begin{pmatrix} 
0\\
1\\
0\\
\end{pmatrix}
\begin{pmatrix}
0\\
0\\
1\\
\end{pmatrix}
= 0 + 0 + 0 = 0\qquad$ <br>

$u = ai + bj + ck = a\begin{pmatrix}
1\\
0\\
0\\
\end{pmatrix} + b\begin{pmatrix}
0\\
1\\
0\\
\end{pmatrix} + c\begin{pmatrix}
0\\
0\\
1\\
\end{pmatrix}\qquad = \begin{pmatrix}
a\\
0\\
0\\
\end{pmatrix} + \begin{pmatrix}
0\\
b\\
0\\
\end{pmatrix} + \begin{pmatrix}
0\\
0\\
c\\
\end{pmatrix}\qquad = \begin{pmatrix}
a\\
b\\
c\\
\end{pmatrix}$ <br>
$v = di + ej + fk = d\begin{pmatrix}
1\\
0\\
0\\
\end{pmatrix} + e\begin{pmatrix}
0\\
1\\
0\\
\end{pmatrix} + f\begin{pmatrix}
0\\
0\\
1\\
\end{pmatrix}\qquad = \begin{pmatrix}
d\\
0\\
0\\
\end{pmatrix} + \begin{pmatrix}
0\\
e\\
0\\
\end{pmatrix} + \begin{pmatrix}
0\\
0\\
f\\
\end{pmatrix}\qquad = \begin{pmatrix}
d\\
e\\
f\\
\end{pmatrix}$ <br>
Then, <br>
$u \cdot v = \begin{pmatrix}
a\\
b\\
c\\
\end{pmatrix} \cdot \begin{pmatrix}
d\\
e\\
f\\
\end{pmatrix} = ad + be + cf$ <b>Hence, proved!</b>

------------------------------------------------------------------------------------------------------

5.Let $u = \begin{pmatrix}
-3\\
2\\
\end{pmatrix}$ and $v = \begin{pmatrix} 
-2\\
-3\\
\end{pmatrix}$ be vector in $\mathbb{R}^2$. Plot these vectors in $\mathbb{R}^2$ and show that the vectors are orthogonal. Hence solve the equation $-3x + 2y = 0$

<b>Solution</b><br>
For orthogonal, $u \cdot v = 0$ <br>
Here, $u \cdot v = (-3)(-2) + 2(-3) = 6-6 = 0$
Therefore, $u$ and $v$ are orthogonal or perpendicular, so infinite choices for $x$ and $y$ in the equation $-3x + 2y = 0$ Generally, $x = 2s$ and $y = 3s$ where, $s \in \mathbb{R}$

---------------------------------------------------------------------------------------

6. Let $u = \begin{pmatrix}
7\\
-2\\
\end{pmatrix}$ and $v = \begin{pmatrix} 
-5\\
3\\
\end{pmatrix}$. Determine the following norms and plot your results on the same axes:

(a)$|| u + v || \quad$ (b) $d(u,v) = || u - v ||$

<b>Solution</b> <br>
(a) $\Vert u + v \rVert = \lVert \begin{pmatrix}
2\\
1\\
\end{pmatrix} \rVert = \sqrt{2^2 + 1^2} = \sqrt5$ <br>
(b) $d(u, v) = \lVert u - v \rVert = \lVert \begin{pmatrix}7 - (-5)\\
-2-3\\
\end{pmatrix}\rVert = \sqrt{12^2 + (-5)^2} = \sqrt{169} = 13$

---------------------------------------------------------

7. Prove properties (ii), (v) and (vii) of proposition 2.1

<b>Solution</b> <br> 
(ii) states $(u + v) + w = u + (v + w)$ <br>
(v) states $k(u + v) = ku + kv$<br>
(vii) states $(kc)\cdot u = k \cdot (cu)$

--------------------------------------

8. Prove property of (i) of Proposition 2.6

<b>Solution</b><br> 
(i) states $(u + v)\cdot = u\cdot w + v\cdot w$

----------------------------------------------------------------------------

9. Determine $\frac{1}{|| u ||}u$ for the following vectors in $\mathbb{R}^n$:

(a)$ u = \begin{pmatrix}
2&-7\\
\end{pmatrix}^T\quad$ (b) $ u = \begin{pmatrix}
-9&3&7\\
\end{pmatrix}^T\quad$ (c) $u = \begin{pmatrix}
-3&5&8&6\\
\end{pmatrix}^T\quad$ (d)$u = \begin{pmatrix}
-6&2&8&3&5\\
\end{pmatrix}^T\quad$

Determine $||\frac{1}{||u||}u||$ in each case.

<b>Solution</b> <br>
<b>(a)</b><br>$\lVert u \rVert = \lVert \begin{pmatrix}
2\\
-7\\
\end{pmatrix}\rVert = \sqrt{2^2 + (-7)^2} = \sqrt{53}$ <br>
So, $\frac{1}{|| u ||}u = \frac{1}{\sqrt{53}} \begin{pmatrix}
2\\
-7\\
\end{pmatrix}$

Also, as $\lVert u \rVert^2 = u \cdot u $. <br>
Here, $\lVert  \frac{1}{|| u ||}u \rVert^2 = \frac{1}{\sqrt{53}}\begin{pmatrix}
2\\
-7\\
\end{pmatrix} \cdot \frac{1}{\sqrt{53}}\begin{pmatrix}
2\\
-7\\
\end{pmatrix}$ <br>
$\qquad \qquad \quad = \frac{1}{53} \cdot (2^2 + (-7)^2)$ <br>
$\qquad \qquad \quad = 1$

Hence, $\lVert  \frac{1}{|| u ||}u \rVert = \sqrt1 = 1$

<b>(b)</b><br>
$\lVert u \rVert = \lVert \begin{pmatrix}
-9\\
3\\
7\\
\end{pmatrix}\rVert = \sqrt{(-9)^2 + (3)^2 + (7)^2} = \sqrt{139}$ <br>
So, $\frac{1}{|| u ||}u = \frac{1}{\sqrt{139}} \begin{pmatrix}
-9\\
3\\
7\\
\end{pmatrix}$

Also, as $\lVert u \rVert^2 = u \cdot u $. <br>
Here, $\lVert  \frac{1}{|| u ||}u \rVert^2 = \frac{1}{\sqrt{139}}\begin{pmatrix}
-9\\
3\\
7\\
\end{pmatrix} \cdot \frac{1}{\sqrt{139}}\begin{pmatrix}
-9\\
3\\
7\\
\end{pmatrix}$ <br>
$\qquad \qquad \quad = \frac{1}{139} \cdot (2^2 + (-7)^2)$ <br>
$\qquad \qquad \quad = 1$

Hence, $\lVert  \frac{1}{|| u ||}u \rVert = \sqrt1 = 1$

<b>(c)</b> <br>$\lVert u \rVert = \lVert \begin{pmatrix}
-3\\
5\\
8\\
6\\
\end{pmatrix}\rVert = \sqrt{(-3)^2 + 5^2 + (8)^2 + 6^2} = \sqrt{134}$ <br>
So, $\frac{1}{|| u ||}u = \frac{1}{\sqrt{134}} \begin{pmatrix}
-3\\
5\\
8\\
6\\
\end{pmatrix}$

Also, as $\lVert u \rVert^2 = u \cdot u $. <br>
Here, $\lVert  \frac{1}{|| u ||}u \rVert^2 = \frac{1}{\sqrt{134}}\begin{pmatrix}
-3\\
5\\
8\\
6\\
\end{pmatrix} \cdot \frac{1}{\sqrt{134}}\begin{pmatrix}
-3\\
5\\
8\\
6\\
\end{pmatrix}$ <br>
$\qquad \qquad \quad = \frac{1}{134} \cdot ((-3)^2 + 5^2 + 8^2 + 6^2)$ <br>
$\qquad \qquad \quad = 1$

Hence, $\lVert  \frac{1}{|| u ||}u \rVert = \sqrt1 = 1$


<b>(d)</b> <br>$\lVert u \rVert = \lVert \begin{pmatrix}
-6\\
2\\
8\\
3\\
5\\
\end{pmatrix}\rVert = \sqrt{(-6)^2 + 2^2 + (8)^2 + 3^2 + 5^2} = \sqrt{138}$ <br>
So, $\frac{1}{|| u ||}u = \frac{1}{\sqrt{138}} \begin{pmatrix}
-6\\
2\\
8\\
3\\
5\\
\end{pmatrix}$

Also, as $\lVert u \rVert^2 = u \cdot u $. <br>
Here, $\lVert  \frac{1}{|| u ||}u \rVert^2 = \frac{1}{\sqrt{138}}\begin{pmatrix}
-6\\
2\\
8\\
3\\
5\\
\end{pmatrix} \cdot \frac{1}{\sqrt{138}}\begin{pmatrix}
-6\\
2\\
8\\
3\\
5\\
\end{pmatrix}$ <br>
$\qquad \qquad \quad = \frac{1}{138} \cdot ((-6)^2 + 2^2 + 8^2 + 3^2 + 5^2)$ <br>
$\qquad \qquad \quad = 1$

Hence, $\lVert  \frac{1}{|| u ||}u \rVert = \sqrt1 = 1$

-----------------------------------------------------------------------------

10. Show that, for any non-zero vector $u$ in $\mathbb{R}^n$, we have  $||\frac{1}{||u||}u|| = 1$

<b>Solution</b><br> 
If we have $u = \begin{pmatrix}
2\\
-7\\
\end{pmatrix}$

Then, <br>
$\lVert u \rVert = \lVert \begin{pmatrix}
2\\
-7\\
\end{pmatrix}\rVert = \sqrt{2^2 + (-7)^2} = \sqrt{53}$ <br>
So, $\frac{1}{|| u ||}u = \frac{1}{\sqrt{53}} \begin{pmatrix}
2\\
-7\\
\end{pmatrix}$

Also, as $\lVert u \rVert^2 = u \cdot u $. <br>
Here, $\lVert  \frac{1}{|| u ||}u \rVert^2 = \frac{1}{\sqrt{53}}\begin{pmatrix}
2\\
-7\\
\end{pmatrix} \cdot \frac{1}{\sqrt{53}}\begin{pmatrix}
2\\
-7\\
\end{pmatrix}$ <br>
$\qquad \qquad \quad = \frac{1}{53} \cdot (2^2 + (-7)^2)$ <br>
$\qquad \qquad \quad = 1$

Hence, $\lVert  \frac{1}{|| u ||}u \rVert = \sqrt1 = 1$

----------------------------------------------------------------------------

11. Let $u$ and $v$ be vectors in $\mathbb{R}^n$. <i>Disprove</i> the following propositions:

(a) If $u \cdot v = 0$ then $u = 0$ or $v = 0$ <br>
(b) $|| u + v|| = ||u|| + ||v||$

<b>Solution</b><br>
<b>(a)</b> If $u = \begin{pmatrix}
-3\\
2\\
\end{pmatrix}$ and $v = \begin{pmatrix}
-2\\
-3\\
\end{pmatrix}$ Then, 
$u \cdot v = \begin{pmatrix}
-3\\
2\\
\end{pmatrix} \cdot  \begin{pmatrix}
-2\\
-3\\
\end{pmatrix}$<br>
Then, $ u \cdot v = (-3)(-2) + 2(-3) = 6 -6 = 0 $. Hence, disproved!

<b>(b)</b> Let $u = \begin{pmatrix}
1\\
2\\
1\\
\end{pmatrix}$ and $v = \begin{pmatrix}
2\\
1\\
3\\
\end{pmatrix}$ 

Then, $\lVert u + v \rVert = \lVert \begin{pmatrix}
3\\
3\\
4\\
\end{pmatrix}\rVert = \sqrt{3^2 + 3^2 + 3^4} = \sqrt{34}$

Here, $\lVert u \rVert = \sqrt{1^2 +2^2 + 1^2} = \sqrt6$ <br>
and $\lVert u \rVert = \sqrt{2^2 + 1^2 + 3^2} = \sqrt{14}$ 

$\sqrt{34} \ne \sqrt6 + \sqrt{14}$. Hence, disproved!

--------------------------------------------------------------

12. Let $u_1, u_2, u_3, ..., u_n$ be orthogonal vectors in $\mathbb{R}^n$. Prove

(i) $|| u_1 + u_2||^2 = ||u_1||^2 + ||u_2||^2$<br>
(ii) $|| u_1 + u_2 + ... + u_n||^2 = ||u_1||^2 + ||u_2||^2 + ... + ||u_n||^2$

<b>Solution</b> <br> 
(i) $\lVert u_1 + u_2 \rVert^2 = (u_1 + u_2) \cdot (u_1 + u_2)$ 

$\qquad \qquad \quad = (u_1 + u_2) \cdot u_1 + (u_1 + u_2) \cdot u_2$ <br>
$\qquad \qquad \quad = u_1 \cdot u_1 + u_2 \cdot u_1 + u_1 \cdot u_2 + u_2 \cdot u_2$ <br>
$\qquad \qquad \quad = \lVert u_1 \rVert^2 + u_2 \cdot u_1 + u_1 \cdot u_2 + \lVert u_2 \rVert^2 $<br>
$\qquad \qquad \quad = \lVert u_1 \rVert^2 + \lVert u_2 \rVert^2$ <br>
Hence, proved

-------------------------------------------------------------------------------------------

13. Let $u$ and $v$ be vectors in $\mathbb{R}^n$. Prove that


(a)$||u + v||^2 + ||u - v||^2 = 2||u||^2 + 2||v||^2$

(b)$||u + v||^2 - ||u - v||^2 = 4(u \cdot v)$

<b>Solution</b> <br>
<b>(a)</b><br> $\Vert u + v \rVert^2 = $ <br>
$\qquad = (u + v) \cdot (u + v)$ <br>
$\qquad = (u + v) \cdot u + (u + v) \cdot v $ <br>
$\qquad = u\cdot u + u \cdot v + u \cdot v + v \cdot v$ <br> 
$\qquad = \lVert u \rVert^2 + 2 u \cdot v + \lVert v\rVert^2$ <br>

Similarly, $\Vert u - v \rVert^2 = $ <br>
$\qquad = (u - v) \cdot (u - v)$ <br>
$\qquad = (u - v) \cdot u + (u - v) \cdot (-v) $ <br>
$\qquad = u\cdot u - v \cdot u + u \cdot (-v) - v \cdot (-v)$ <br> 
$\qquad = \lVert u \rVert^2 - 2 u \cdot v + \lVert v\rVert^2$ <br>

Therefore, $\Vert u + v \rVert^2 + \Vert u - v \rVert^2 = \lVert u \rVert^2 + 2 u \cdot v + \lVert v\rVert^2 + \lVert u \rVert^2 - 2 u \cdot v + \lVert v\rVert^2$ 

$\Rightarrow \lVert u + v\rVert^2 + \Vert u - v\rVert^2 = 2\Vert u\rVert^2 + 2\lVert v\rVert^2$

<b>(b)</b> <br>
Taking $\lVert u + v\rVert^2$ and  $\Vert u - v\rVert^2$ from above, we have: 

$\Vert u + v \rVert^2 - \Vert u - v \rVert^2 = \lVert u \rVert^2 + 2 u \cdot v + \lVert v\rVert^2 - (\lVert u \rVert^2 - 2 u \cdot v + \lVert v\rVert^2)$


$\qquad \qquad \qquad \qquad =  \lVert u \rVert^2 + 2 u \cdot v + \lVert v\rVert^2 - \lVert u \rVert^2 + 2 u \cdot v - \lVert v\rVert^2)$


$\Rightarrow$ Therefore, $\Vert u + v \rVert^2 - \Vert u - v \rVert^2 = 4( u \cdot v)$

-------------------------------------------------------------------------------------------

14. This question is on the properties of the distance function $d(u,v)$ where $u$ and $v$ are vectors in n-space.

(i) Show that $d(u,v) = \sqrt{(u_1 - v_1)^2 + (u_2 - v_2)^2 + ... + (u_n - v_n)^2}$<br>
(ii) Prove that $d(u,v) = d(v,u)$ <br>
(iii) Prove that $d(u,v) \ge 0$ and $d(u,v) = 0 \iff u = v$

<b>Solution</b> <br>

(i) We know that, <br>
$\qquad d(u, v) = \lVert u - v \rVert = \sqrt{(u - v) \cdot (u - v)}$

If $u$ and $v$ goes upto $n-$term, we have 

$ u - v = \begin{pmatrix}
u_1 - v_1\\
u_2 - v_2\\
\vdots - \vdots\\
u_n - v_n\\
\end{pmatrix}$

Then, <br>
$d(u, v) = \lVert u - v \rVert = \sqrt{\begin{pmatrix}
u_1 - v_1\\
u_2 - v_2\\
\vdots - \vdots\\
u_n - v_n\\
\end{pmatrix}\cdot \begin{pmatrix}
u_1 - v_1\\
u_2 - v_2\\
\vdots - \vdots\\
u_n - v_n\\
\end{pmatrix}}$

$ d(u, v) = \sqrt{(u_1 - v_1)^2 + (u_2 + v_2)^2 + \dots + (u_n - v_n)^2}$

Hence, proved

(ii) $ d(u, v) = \sqrt{(u_1 - v_1)^2 + (u_2 + v_2)^2 + \dots + (u_n - v_n)^2}$


$\qquad= \sqrt{(v_1 - u_1)^2 + (v_2 + u_2)^2 + \dots + (v_n - u_n)^2} \quad$ (fippling inside bracket that gets squared do not make difference) 

$\qquad=d(v,u)$


```python

```
